Flapjack/Test/Lab.lean
@@ -1,0 +1,39 @@
+import Flapjack.Lab
+
+namespace Flapjack
+
+example :
+    labFlatten false 20 7 [] []
+      (.ffi "sum" 1 2 3 4 9 : StackProg Nat) =
+      { lines := [
+          .labAsm (.locValue 9 ⟨20, 7⟩) [] 0,
+          .labAsm (.callFfi "sum") [] 0,
+          .label 20 7 0],
+        terminal := false,
+        nextLabel := 8 } := by
+  simp [labFlatten, labLabel]
+
+example :
+    labFlatten false 3 4 [] []
+      (.loop (.seq (.tick) (.break 0)) : StackProg Nat) =
+      { lines := [
+          .label 3 4 0,
+          .asm .tick [] 0,
+          .labAsm (.jump ⟨3, 5⟩) [] 0,
+          .labAsm (.jump ⟨3, 4⟩) [] 0,
+          .label 3 5 0],
+        terminal := false,
+        nextLabel := 6 } := by
+  simp [labFlatten, labLabel, labJump, labFindLabel]
+
+example :
+    labProgramToSection 2 3
+      (.seq (.tick) (.return 4) : StackProg Nat) =
+      ⟨2, [
+        .asm .tick [] 0,
+        .label 2 1 0,
+        .asm (.jumpReg 4) [] 0,
+        .label 2 3 0]⟩ := by
+  simp [labProgramToSection, labFlatten, labIsSequence, labLabel]
+
+end Flapjack
