Flapjack/Tests.lean
@@ -13,6 +13,7 @@ import Flapjack.Test.Structured
 import Flapjack.Test.CorrectnessFfi
 import Flapjack.Test.Ffi
 import Flapjack.Test.Stack
+import Flapjack.Test.Lab
 
 /-!
 # Flapjack regression tests
